src/program_proof/tulip/paxos/invariance/ascend.v
@@ -43,24 +43,28 @@ Section ascend.
     by iDestruct (big_sepM_lookup with "Hpsaubs") as "?"; first apply Hfixed.
   Qed.
 
-  Lemma paxos_inv_ascend γ nids nid termc terml v v' :
+  Lemma paxos_inv_ascend {γ nids nid termc terml lsnc v} v' :
     nid ∈ nids ->
     is_term_of_node nid termc ->
     (terml < termc)%nat ->
+    (lsnc ≤ length v')%nat ->
+    prefix (take lsnc v) v' ->
     safe_base_proposal_by_length γ nids termc v' -∗
     own_current_term_half γ nid termc -∗
     own_ledger_term_half γ nid terml -∗
+    own_committed_lsn_half γ nid lsnc -∗
     own_node_ledger_half γ nid v -∗
     paxos_inv γ nids ==∗
     own_current_term_half γ nid termc ∗
     own_ledger_term_half γ nid termc ∗
+    own_committed_lsn_half γ nid lsnc ∗
     own_node_ledger_half γ nid v' ∗
     paxos_inv γ nids ∗
     own_proposal γ termc v' ∗
     is_base_proposal_receipt γ termc v' ∗
     is_accepted_proposal_lb γ nid termc v'.
   Proof.
-    iIntros (Hnid Hton Hlt) "#Hsafelen Htermc Hterml Hv Hinv".
+    iIntros (Hnid Hton Hlt Hlsncub Hlsnc) "#Hsafelen Htermc Hterml Hlsnc Hv Hinv".
     iNamed "Hinv".
     iAssert (safe_base_proposal γ nids termc v')%nat as "#Hsafe".
     { iNamed "Hsafelen". iNamed "Hvotes".
@@ -160,9 +164,11 @@ Section ascend.
     (* Extract witness of the inserted proposal to re-establish the node invariant. *)
     iDestruct (proposal_witness with "Hp") as "#Hplb".
     (* Re-establish node invariant. *)
-    iMod (node_inv_advance v' with "[] [] Htermc Hterml Hv Hnode")
-      as "(Htermc & Hterml & Hv & Hnode & #Hacptlb)".
+    iMod (node_inv_advance v' with "[] [] Htermc Hterml Hlsnc Hv Hnode")
+      as "(Htermc & Hterml & Hlsnc & Hv & Hnode & #Hacptlb)".
     { apply Hlt. }
+    { apply Hlsncub. }
+    { apply Hlsnc. }
     { by iFrame "Hpsbrcp". }
     { by iFrame "Hplb". }
     iDestruct (big_sepM_insert_2 with "Hnode Hnodes") as "Hnodes".
