src/program_proof/tulip/paxos/invariance/expand.v
@@ -1,0 +1,57 @@
+From Perennial.program_proof.tulip.paxos Require Import prelude.
+
+Section expand.
+  Context `{!paxos_ghostG Σ}.
+
+  Lemma node_inv_expand γ nids nid terml lsnc logn lsnc' :
+    (lsnc ≤ lsnc')%nat ->
+    (lsnc' ≤ length logn)%nat ->
+    safe_ledger_above γ nids terml (take lsnc' logn) -∗
+    own_committed_lsn_half γ nid lsnc -∗
+    own_node_ledger_half γ nid logn -∗
+    node_inv γ nids nid terml ==∗
+    own_committed_lsn_half γ nid lsnc' ∗
+    own_node_ledger_half γ nid logn ∗
+    node_inv γ nids nid terml.
+  Proof.
+    iIntros (Hge Hle) "#Hcmted HlsncX HlognX Hinv".
+    iNamed "Hinv".
+    (* Agreements. *)
+    iDestruct (committed_lsn_agree with "HlsncX Hlsnc") as %->.
+    iDestruct (node_ledger_agree with "HlognX Hlogn") as %->.
+    (* Update the committed LSN. *)
+    iMod (committed_lsn_update lsnc' with "HlsncX Hlsnc") as "[HlsncX Hlsnc]".
+    iClear "Hsafel".
+    by iFrame "∗ # %".
+  Qed.
+
+  Lemma paxos_inv_expand {γ nids nid terml lsnc logn} lsnc' :
+    nid ∈ nids ->
+    (lsnc ≤ lsnc')%nat ->
+    (lsnc' ≤ length logn)%nat ->
+    safe_ledger_above γ nids terml (take lsnc' logn) -∗
+    own_ledger_term_half γ nid terml -∗
+    own_committed_lsn_half γ nid lsnc -∗
+    own_node_ledger_half γ nid logn -∗
+    paxos_inv γ nids ==∗
+    own_ledger_term_half γ nid terml ∗
+    own_committed_lsn_half γ nid lsnc' ∗
+    own_node_ledger_half γ nid logn ∗
+    paxos_inv γ nids.
+  Proof.
+    iIntros (Hnid Hge Hle) "#Hsafel Hterml Hlsnc Hlogn Hinv".
+    iNamed "Hinv".
+    rewrite -Hdomtermlm elem_of_dom in Hnid.
+    destruct Hnid as [terml' Hnid].
+    iDestruct (big_sepM_lookup_acc _ _ nid with "Hnodes") as "[Hnode HnodesC]".
+    { apply Hnid. }
+    iDestruct (own_ledger_term_node_inv_terml_eq with "Hterml Hnode") as %->.
+    (* Re-establish the node invariant. *)
+    iMod (node_inv_expand with "Hsafel Hlsnc Hlogn Hnode") as "(Hlsnc & Hlogn & Hnode)".
+    { apply Hge. }
+    { apply Hle. }
+    iDestruct ("HnodesC" with "Hnode") as "Hnodes".
+    by iFrame "∗ # %".
+  Qed.
+
+End expand.
